

$$X_t = \begin{bmatrix} x_t \\ y_t \\ \theta_t \end{bmatrix}, u_t = \begin{bmatrix} v_x \\ \omega_z \end{bmatrix}$$

$$v_R = r\omega_R, v_L = r\omega_L \sim v_x = \frac{v_R + v_L}{2}, \omega_z = \frac{v_R - v_L}{w}$$

$$\begin{aligned} v_R &= v_x + \frac{w}{2} \omega_z \\ v_L &= v_x - \frac{w}{2} \omega_z \end{aligned}$$

## Motion Model

از طرفی ال motion model را می‌توان نوشت به صورت زیر:

$$\frac{dx}{dt} = v_x \cos \theta, \frac{dy}{dt} = v_x \sin \theta, \frac{d\theta}{dt} = \omega_z$$

حال:

$$\begin{aligned} x_t &= x_{t-1} + v_x \cos \theta_{t-1} \Delta t, y_t = y_{t-1} + v_x \sin \theta_{t-1} \Delta t \\ \theta_t &= \theta_{t-1} + \omega_z \Delta t \end{aligned}$$

$$X_t = f(X_{t-1}, u_{t-1}) + \varepsilon_t, \varepsilon_t \sim \mathcal{N}(0, R_t)$$

## Measurement Model

Visual Odometry  $\rightarrow (\Delta x, \Delta y)$   
 IMU  $\rightarrow \theta$

$$Y_t = \begin{bmatrix} \Delta x_t \\ \Delta y_t \\ \theta_t \end{bmatrix}$$

$$\Delta x_t = x_t - x_{t-1}, \Delta y_t = y_t - y_{t-1}, \theta_t = \theta_t$$

$$Y_t = h(X_t) + \delta_t, \delta_t \sim \mathcal{N}(0, R_t)$$

$$h(X_t) = \begin{bmatrix} x_t - x_{t-1} \\ y_t - y_{t-1} \\ \theta_t \end{bmatrix}$$

$$F_t = \frac{\partial f}{\partial X} = \begin{bmatrix} 1 & 0 & -v_y \sin \theta \Delta t \\ 0 & 1 & v_x \cos \theta \Delta t \\ 0 & 0 & 1 \end{bmatrix}$$

: EKF

$$\bar{\Sigma}_t = F_t \Sigma_{t-1} F_t^T + Q_t$$

measurement Model  $\rightarrow \begin{bmatrix} \hat{x}_{t|t-1} - u_{t-1} \\ \hat{y}_{t|t-1} - y_{t-1} \\ \hat{\theta}_{t|t-1} \end{bmatrix} \sim \frac{\partial h}{\partial X} = \begin{bmatrix} 1 & 0 & 0 \\ 0 & 1 & 0 \\ 0 & 0 & 1 \end{bmatrix} = H_t \cdot I$

$$z_t = y_t - \hat{y}_t \sim K_t \cdot \bar{\Sigma}_t H_t^T (H_t \bar{\Sigma}_t H_t^T + Q_t)^{-1} \\ \sim \hat{X}_{t|t} = \hat{X}_{t|t-1} + K_t z_t$$

$$\Sigma_t = (I - K_t H_t) \bar{\Sigma}_t$$